coq/Equivalences.v
@@ -395,7 +395,6 @@ Qed.
 
 
 
-
 End object.
 
 
